We are going to solve the equation (\ref{PDE}) when $\beta = 1$ and $\kappa = 0$, i.e.,
\begin{equation}
	\partial_t V + \frac{1}{2}\sigma^2 S^2 \partial_{SS}V -r V + C\exp{rt}= 0.
\end{equation}

To do so, we are going to try the method of variables separation, i.e., let's suppose that 
\begin{equation}
	V(S,t) = F(S)G(t) + g(t);
\end{equation}
but firstly we will find the solution for the honogeneous equation $V(S,t) = F(S)G(t)$. Note that
$$
	\begin{aligned}
		F(S) G'(t) + \frac{1}{2}\sigma^2 S^2 F''(S)G(t) - r F(S)G(t)			 &= 0 \\
		F(S) G'(t) + \left(\frac{1}{2}\sigma^2 S^2 F''(S) - r F(S)\right) G(t) 	&= 0\\
		\frac{rF(S) - \frac{1}{2}\sigma^2S^2 F''(S)}{F(S)}						&=  \frac{G'(t)}{G(t)}\\
		r - \frac{1}{2}\sigma^2 S^2 \frac{F''(S)}{F(S)} 						&=  \frac{G'(t)}{G(t)},
	\end{aligned}
$$
and since there is an equality of functions depending on different variables, they are equal to a constant, say $M$, i.e., 
$$
	\begin{aligned}
			r - \frac{1}{2}\sigma^2 S^2 \frac{F''(S)}{F(S)}  	&= M \\
			 \frac{2(r-M)}{\sigma^2}\cdot \frac{1}{S^2} 			&= \frac{F''(S)}{F(S)},
	\end{aligned}
$$
which is solved by an exponential function $F(S) = S^a$ with a constant $a$,
$$
	\begin{aligned}
		 \frac{2(r-M)}{\sigma^2}\cdot \frac{1}{\cancel{S^2}} 			&= \frac{a(a-1)}{\cancel{S^2}}\\
		 a^2 - a +  \frac{2(M-r)}{\sigma^2} &= 0,
	\end{aligned}
$$
i.e., 
\begin{equation}
	a = \frac{1\pm\sqrt{1+8\frac{(r-M)}{\sigma^2}}}{2}
\end{equation}
On the other hand,
$$
	G(t) = C_G \exp{M t}.
$$

Finally, from $V(S,t) = F(S)G(t) + g(t)$ we obtain
$$
	\begin{aligned}
			F(S) G'(t) + g'(t) + \frac{1}{2}\sigma^2 S^2 F''(S)G(t) - r F(S)G(t)	+ C\exp{rt}		 &= 0\\
			g'(t) + C\exp{rt} &= 0\\
			g'(t) &= -C\exp{rt},
	\end{aligned}
$$ 
and then
\begin{equation}
	g(t) = - N \frac{C}{r}\exp{rt},
\end{equation}
which implies
\begin{equation}
	V(S,t) = S^a  C_G \exp{M t} - N \frac{C}{r}\exp{rt},. 
\end{equation}

We know that $V(S,T) = \max(F, RS)$, and therefore, for large $S$, $V(S,T) = RS$, i.e., 
$$
		V(S,t) = S^a  C_G \exp{M T} - N \frac{C}{r}\exp{rT} = RS,
$$
i.e., 
$$
	\begin{cases}
		a &= 1\\
		C_G \exp{MT} &= 1\\
		N\frac{C}{r}e^{rT} &= 0
	\end{cases},
$$
from which we obtain that $N = 0$, $C_G = \exp{-MT}$ and $M = r$, i.e., 
\begin{equation}
	V(S,t) = S \exp{-r(T-t)}
\end{equation}